WIP

OptSim.v
@@ -13,11 +13,28 @@ From RelationAlgebra Require Import
 
 Import CoindNotations.
 
+Lemma itr_unfold_l `{laws} `{KA ≪ l} :
+  forall (n : ob X) (x : X n n), x^+ ≡ x + x⋅x^+.
+Proof.
+  intros. now rewrite itr_str_l, str_unfold_l, <- itr_str_l, dotxpls, dotx1 at 1.
+Qed.
+
+Lemma itr_unfold_r `{laws} `{KA ≪ l} :
+  forall (n : ob X) (x : X n n), x^+ ≡ x + x^+⋅x.
+Proof.
+  intros. now rewrite itr_str_r, kleene.str_unfold_r, <- itr_str_r, dotplsx, dot1x at 1.
+Qed.
+
+Lemma str_itr' `{laws} `{KA ≪ l} :
+  forall (n : ob X) (x : X n n), x^+ ≦ x^*.
+Proof.
+  intros. now rewrite str_itr, <- leq_cup_r.
+Qed.
 
 Module SimOpt.
 
-  Variant compress_opt := compress_ind | compress_coind | nocompress.
-  Definition div := compress_ind.
+  Variant compress_opt := compress_mut | compress_coind | nocompress.
+  Definition div := compress_mut.
   Variant lock_opt := lock | nolock.
   Variant expand_opt := expand | noexpand.
   Variant ub_opt := noub | ub | ttub. (* TODO can non-TT UB be characterized just as "every transition is possible"? *)
@@ -35,6 +52,36 @@ Record LTS := {
   ub_state : St -> Prop;
 }.
 
+(*Section LockLTS.
+
+  Context (lts : LTS).
+  Variant LockObservable := | Event (e : lts.(Observable)) | NoEvent.
+  Program Definition LockSt := {| type_of := (bool * lts.(St))%type |}.
+  Variant locktrans : @label LockObservable -> LockSt -> LockSt -> Prop :=
+  | locktrans_ev b o s t : lts.(trans) (obs o) s t -> locktrans (obs (Event o)) (b, s) (true, t)
+  | locktrans_noev s : (forall l t, lts.(trans) l s t -> False) -> locktrans (obs NoEvent) (true, s) (true, s)
+  .
+  Definition lockepsilon : LockSt -> LockSt -> Prop :=
+    fun '(b, s) '(b', s') =>
+    lts.(epsilon) s s' /\ (
+      (b = false /\ b' = false) \/
+      (b = true /\ b' = false) \/
+      (b = true /\ b' = true /\ forall l s'', lts.(trans) l s s'' -> False)
+    ).
+  Definition LockRobs : LockObservable -> LockObservable -> Prop. Admitted.
+  Definition lock_ub_state : LockSt -> Prop. Admitted.
+
+  Definition lock := {|
+    Observable := LockObservable;
+    St := LockSt;
+    trans := locktrans;
+    epsilon := lockepsilon;
+    Robs := LockRobs;
+    ub_state := lock_ub_state
+  |}.
+
+End LockLTS.*)
+
 Section WithLTS.
 
 Context (lts : LTS).
@@ -45,27 +92,6 @@ Let epsilon := lts.(epsilon).
 Let Robs := lts.(Robs).
 Let ub_state := lts.(ub_state).
 Let label := @label Observable.
-
-(*Module LockLTS.
-
-  Variant Observable := | Event (e : LTS.Observable) | NoEvent.
-  Definition St := (bool * LTS.St)%type.
-  Variant trans : @label Observable -> St -> St -> Prop :=
-  (*| trans_ev l s t : LTS.trans l s t -> trans (Event l) s t*)
-  | trans_noev s : (forall l t, LTS.trans l s t -> False) -> trans (obs NoEvent) (true, s) (true, s)
-  .
-  Definition epsilon : St -> St -> Prop :=
-    fun '(b, s) '(b', s') =>
-    LTS.epsilon s s' /\ (
-      (b = false /\ b' = false) \/
-      (b = true /\ b' = false) \/
-      (b = true /\ b' = true /\ forall l s'', LTS.trans l s s'' -> False)
-    ).
-  Definition Robs : Observable -> Observable -> Prop. Admitted.
-  Definition ub_state : St -> Prop. Admitted.
-  (*Parameter eq : St -> St -> Prop.*)
-
-End LockLTS.*)
 
 #[global] Instance : Proper (weq ==> eq ==> eq ==> iff) (hrel_of (n := St) (m := St)).
 Proof.
@@ -99,6 +125,10 @@ Qed.
 
 Definition diverges := gfp divergesF.
 
+#[export] Instance : Proper (St.(Eq) ==> flip impl) diverges.
+Proof.
+Admitted.
+
 Variant extrans (st : St) : Prop :=
 trans_intro l st' : trans l st st' -> extrans st.
 Hint Constructors extrans : optsim.
@@ -123,6 +153,39 @@ Context (compress : SimOpt.compress_opt)
   (expand : SimOpt.expand_opt)
   (ub : SimOpt.ub_opt).
 
+Variant DTauAnswer (R Rind : relation St) s' t : Prop :=
+| dtau_match t' (TR : trans tau t t') (DIV : R s' t')
+| dtau_div (DIV : Rind s' t)
+.
+
+Definition divpresIndF R Rind s t :=
+  forall s', trans tau s s' -> DTauAnswer R Rind s' t.
+
+Section NoElim.
+#[local] Unset Elimination Schemes.
+Inductive divpresInd R s t : Prop :=
+| divpresI : divpresIndF R (divpresInd R) s t -> divpresInd R s t.
+End NoElim.
+
+Definition divpresInd_ind :
+  forall R P : St -> St -> Prop,
+       (forall s t : St,
+         (divpresIndF R (fun s t => divpresInd R s t /\ P s t) s t) -> 
+        P s t) -> forall t t0 : St, divpresInd R t t0 -> P t t0.
+Proof.
+  intros until 1. fix F 3. intros. apply H. destruct H0.
+  red. intros. apply H0 in H1 as [].
+  - eleft; eauto.
+  - eright; eauto.
+Qed.
+
+Program Definition divpresF : mon (St -> St -> Prop) :=
+{| body R s t := divpresInd R s t |}.
+Next Obligation.
+  induction H0. constructor. intros ??.
+  apply H0 in H1 as []. eleft; eauto. eright; eauto. apply DIV.
+Qed.
+
 Variant ObsAnswer (R : relation St) s' t o : Prop :=
 | ans_obs o' t' (TR : trans (obs o') t t') (SIM : R s' t') (OBS : Robs o o') : ObsAnswer R s' t o
 | ans_delay_obs o' t' (_ : expand = SimOpt.expand) (TR : ((trans tau)^* ⋅ trans (obs o')) t t') (SIM : R s' t') (OBS : Robs o o') : ObsAnswer R s' t o
@@ -138,29 +201,29 @@ Proof.
 Qed.
 
 (* delay/freeze *)
-Variant TauAnswer (R Rind : relation St) s' t : Prop :=
+Variant TauAnswer (R : relation St) Rdiv s' t : Prop :=
 | tau_exact t' (TR : trans tau t t') (SIM : R s' t')
 | tau_compress (_ : compress = SimOpt.compress_coind) (SIM : R s' t)
-| tau_div (_ : compress = SimOpt.compress_ind) (SIM : Rind s' t)
+| tau_div (_ : compress = SimOpt.compress_mut) (SIM : R s' t) (DIV : divpresF Rdiv s' t)
 | tau_expand t' (_ : expand = SimOpt.expand) (TR : (trans tau)^+ t t') (SIM : R s' t')
 .
 Hint Constructors TauAnswer : optsim.
 
-#[export] Instance : forall R Rind,
+#[export] Instance : forall R Rdiv,
   Proper (St.(Eq) ==> St.(Eq) ==> iff) R ->
-  Proper (St.(Eq) ==> St.(Eq) ==> iff) Rind ->
-  Proper (St.(Eq) ==> St.(Eq) ==> flip impl) (TauAnswer R Rind).
+  Proper (St.(Eq) ==> St.(Eq) ==> iff) Rdiv ->
+  Proper (St.(Eq) ==> St.(Eq) ==> flip impl) (TauAnswer R Rdiv).
 Proof.
   intros. cbn. intros.
   destruct H3; rewrite <- ?H1, <- ?H2 in *; eauto with optsim.
-Qed.
+Admitted.
 
 Lemma tau_weak :
   compress = SimOpt.compress_coind ->
   expand = SimOpt.expand ->
-  forall R Rind s' t t',
+  forall R Rdiv s' t t',
   Proper (St.(Eq) ==> St.(Eq) ==> iff) R ->
-  (trans tau)^* t t' -> R s' t' -> TauAnswer R Rind s' t.
+  (trans tau)^* t t' -> R s' t' -> TauAnswer R Rdiv s' t.
 Proof.
   intros -> -> * ? TR SIM.
   rewrite str_itr in TR. destruct TR as [TR | TR].
@@ -169,18 +232,18 @@ Proof.
 Qed.
 
 Lemma tau_weak_div :
-  compress = SimOpt.compress_ind ->
+  compress = SimOpt.compress_mut ->
   expand = SimOpt.expand ->
-  forall R Rind s' t t',
-  Proper (St.(Eq) ==> St.(Eq) ==> iff) Rind ->
-  subrelation Rind R ->
-  (trans tau)^* t t' -> Rind s' t' -> TauAnswer R Rind s' t.
+  forall R Rdiv s' t t',
+  Proper (St.(Eq) ==> St.(Eq) ==> iff) R ->
+  Proper (St.(Eq) ==> St.(Eq) ==> iff) Rdiv ->
+  (trans tau)^* t t' -> R s' t' -> divpresF Rdiv s' t' -> TauAnswer R Rdiv s' t.
 Proof.
-  intros -> -> * ?? TR SIM.
+  intros -> -> * ?? TR SIM DIV.
   rewrite str_itr in TR. destruct TR as [TR | TR].
-  - cbn in TR. apply tau_div; auto. now rewrite TR.
+  - cbn in TR. apply tau_div; auto. now rewrite TR. admit.
   - eapply tau_expand; eauto.
-Qed.
+Admitted.
 
 Definition RL l l' :=
   match l, l' with
@@ -189,7 +252,49 @@ Definition RL l l' :=
   | _, _ => False
   end.
 
-Variant SimAnswer (R Rind : relation St) s' t l : Prop :=
+Section SimInd.
+
+  Variant TauIndAnswer (R Rind : relation St) s' t : Prop :=
+  | taui_exact t' (TR : trans tau t t') (SIM : R s' t')
+  | taui_compress (_ : compress = SimOpt.compress_coind) (SIM : R s' t)
+  | taui_div (_ : compress = SimOpt.compress_mut) (SIM : Rind s' t)
+  | taui_expand t' (_ : expand = SimOpt.expand) (TR : (trans tau)^+ t t') (SIM : R s' t')
+  .
+  Hint Constructors TauIndAnswer : optsim.
+
+  Definition simIndF R Rind s t :=
+    (forall o s', trans (obs o) s s' ->
+      ObsAnswer R s' t o
+    ) /\
+    (forall s', trans tau s s' ->
+      TauIndAnswer R Rind s' t
+    ) /\
+    (lock = SimOpt.nolock \/ (is_stuck s -> is_stuck t)).
+
+  Section NoElim.
+  #[local] Unset Elimination Schemes.
+  Inductive simInd R s t : Prop :=
+  | simI :
+    simIndF R (simInd R) s t -> simInd R s t.
+  End NoElim.
+
+  Definition simInd_ind :
+    forall R P : St -> St -> Prop,
+         (forall s t : St,
+           (simIndF R (fun s t => simInd R s t /\ P s t) s t) -> 
+          P s t) -> forall t t0 : St, simInd R t t0 -> P t t0.
+  Proof.
+    intros until 1. fix F 3. intros. apply H. destruct H0. repeat split; intros.
+    - apply H0 in H1 as [].
+      eleft; eauto.
+      eright; eauto.
+    - apply H0 in H1 as []; esim.
+    - apply H0.
+  Qed.
+
+End SimInd.
+
+(*Variant SimAnswer (R Rind : relation St) s' t l : Prop :=
 | ans_exact l' t' (TR : trans l' t t') (SIM : R s' t') (LBL : RL l l')
 | ans_compress (_ : compress = SimOpt.compress_coind) (SIM : R s' t) (LBL : l = tau)
 | ans_div (_ : compress = SimOpt.compress_ind) (SIM : Rind s' t) (LBL : l = tau)
@@ -204,34 +309,9 @@ Hint Constructors SimAnswer : optsim.
 Proof.
   intros. cbn. intros. subst.
   destruct H4; rewrite <- ?H1, <- ?H2 in *; eauto with optsim.
-Qed.
+Qed.*)
 
-Definition simIndF R Rind s t :=
-  (forall o s', trans (obs o) s s' -> ObsAnswer R s' t o) /\
-  (forall s', trans tau s s' -> TauAnswer R Rind s' t) /\
-  (lock = SimOpt.nolock \/ (is_stuck s -> is_stuck t)) (* FIXME tau* in answer *).
-
-Section NoElim.
-#[local] Unset Elimination Schemes.
-Inductive simInd R s t : Prop :=
-| simI :
-  simIndF R (simInd R) s t -> simInd R s t.
-End NoElim.
-
-Definition simInd_ind :
-  forall R P : St -> St -> Prop,
-       (forall s t : St,
-         (simIndF R (fun s t => simInd R s t /\ P s t) s t) -> 
-        P s t) -> forall t t0 : St, simInd R t t0 -> P t t0.
-Proof.
-  intros until 1. fix F 3. intros. apply H. destruct H0. repeat split; intros.
-  - apply H0 in H1 as [].
-    eleft; eauto.
-    eright; eauto.
-  - apply H0 in H1 as []; esim.
-  - apply H0.
-Qed.
-
+(*
 Definition sim_alt R s t :=
   (forall l s', trans l s s' ->
     match l with
@@ -254,24 +334,6 @@ Qed.
 Definition sim_alt' R s t :=
   (forall l s', trans l s s' -> SimAnswer R (simInd R) s' t l) /\
   (lock = SimOpt.nolock \/ (is_stuck s -> is_stuck t)).
-
-Lemma itr_unfold_l `{laws} `{KA ≪ l} :
-  forall (n : ob X) (x : X n n), x^+ ≡ x + x⋅x^+.
-Proof.
-  intros. now rewrite itr_str_l, str_unfold_l, <- itr_str_l, dotxpls, dotx1 at 1.
-Qed.
-
-Lemma itr_unfold_r `{laws} `{KA ≪ l} :
-  forall (n : ob X) (x : X n n), x^+ ≡ x + x^+⋅x.
-Proof.
-  intros. now rewrite itr_str_r, kleene.str_unfold_r, <- itr_str_r, dotplsx, dot1x at 1.
-Qed.
-
-Lemma str_itr' `{laws} `{KA ≪ l} :
-  forall (n : ob X) (x : X n n), x^+ ≦ x^*.
-Proof.
-  intros. now rewrite str_itr, <- leq_cup_r.
-Qed.
 
 Lemma sim_alt'_equiv : forall R s t, sim_alt R s t <-> sim_alt' R s t.
 Proof.
@@ -301,44 +363,324 @@ Proof.
     destruct SIM. esim.
   - apply H0.
 Qed.
+*)
 
 Program Definition simF :
-  mon (St -> St -> Prop) :=
-{| body R s t :=
-  simInd R s t
+  mon (bool -> St -> St -> Prop) :=
+{| body R b s t :=
+  (b = false -> divpresF (R false) s t) /\
+  (b = true -> (forall o s', trans (obs o) s s' -> ObsAnswer (R true) s' t o) /\
+  (forall s', trans tau s s' -> TauAnswer (R true) (R false) s' t) /\
+  (lock = SimOpt.nolock \/ (is_stuck s -> is_stuck t)) (* FIXME tau* in answer *))
 |}.
 Next Obligation.
-  eapply simInd_mon. 2: apply H0. cbn. apply H.
-Qed.
+  repeat split; intros.
+  - eapply (Hbody divpresF). 2: { apply H0. auto. } cbn. intros. now apply H.
+  - apply H1 in H3 as []; esim.
+  - apply H1 in H3 as []; esim. admit.
+  - now apply H1.
+Admitted.
 
 #[export] Instance simF_eq R :
-  Proper (Eq St ==> Eq St ==> iff) R ->
-  Proper (Eq St ==> Eq St ==> flip impl) (simInd R).
+  Proper (eq ==> Eq St ==> Eq St ==> iff) R ->
+  Proper (eq ==> Eq St ==> Eq St ==> flip impl) (simF R).
 Proof.
-  intros. cbn. intros. revert x x0 H0 H1. induction H2. intros. destruct H0 as (? & ? & ?).
-  constructor. repeat split; intros; rewrite ?H1, ?H2 in * |- *; auto.
-  apply H3 in H5. destruct H5; rewrite <- ?H1, <- ?H2 in * |- *; eauto with optsim.
-  econstructor 3; auto. destruct SIM. apply H7; auto.
-Qed.
+  intros. cbn. intros. subst. destruct H3, y; split; intro; try discriminate.
+  - specialize (H3 eq_refl). destruct H3 as (? & ? & ?).
+    repeat split; intros; rewrite ?H1, ?H2 in * |- *; auto.
+  - admit.
+Admitted.
 
 #[export] Instance Chain_simF_eq : forall (R : Chain simF),
-  Proper (Eq St ==> Eq St ==> iff) ` R.
+  Proper (eq ==> Eq St ==> Eq St ==> iff) ` R.
 Proof.
   intro. apply tower. {
-    intros ? INC ??????. split; intros ???.
-    - eapply INC. assumption.
+    intros ? INC ?? <- ??????. split; intros ???.
+    - eapply INC. assumption. reflexivity.
       now rewrite <- H. now rewrite <- H0.
       now apply H1.
-    - eapply INC. assumption.
+    - eapply INC. assumption. reflexivity.
       now rewrite H. now rewrite H0.
       now apply H1.
   }
-  intros. split; intro.
-  now rewrite H0, H1 in H2.
-  now rewrite H0, H1.
+  intros. split; intro; subst.
+  now rewrite H1, H2 in H3.
+  now rewrite H1, H2.
 Qed.
 
 Definition sim := gfp simF.
+
+Program Definition divsimF lock : mon (St -> St -> Prop) :=
+{|
+  body := fun R s t => (forall o s', ((trans tau)^* ⋅ trans (obs o)) s s' ->
+    exists o' t',
+        ((trans tau)^* ⋅ trans (obs o')) t t' /\
+      R s' t' /\
+      Robs o o') /\
+  (forall s', (trans tau)^* s s' ->
+    exists t', 
+      (trans tau)^* t t' /\ R s' t') /\
+  (diverges s -> diverges t) /\
+  (lock = SimOpt.nolock \/ (is_stuck s -> is_stuck t))
+|}.
+Next Obligation.
+  repeat split; intros; auto.
+  - apply H0 in H4 as (? & ? & ? & ? & ?). eauto 6.
+  - apply H1 in H4 as (? & ? & ?). eauto.
+Qed.
+
+Definition divsim := gfp (divsimF SimOpt.nolock).
+
+Program Definition divsimF' : mon (St -> St -> Prop) :=
+{|
+  body := fun R s t => (forall o s', trans (obs o) s s' ->
+    exists o' t',
+        ((trans tau)^* ⋅ trans (obs o')) t t' /\
+      R s' t' /\
+      Robs o o') /\
+  (forall s', trans tau s s' ->
+    exists t', 
+      (trans tau)^* t t' /\ R s' t') /\
+  (diverges s -> diverges t)
+|}.
+Next Obligation.
+  repeat split; intros; auto.
+  - apply H0 in H3 as (? & ? & ? & ? & ?). eauto 6.
+  - apply H1 in H3 as (? & ? & ?). eauto.
+Qed.
+
+Definition divsim' := gfp divsimF'.
+
+Lemma chain_div : forall (R : Chain simF) s t,
+  diverges t ->
+  simF `R false s t.
+Proof.
+  intro. apply tower. {
+    intros ???????. apply H; auto.
+  }
+  clear R. intros R **.
+  cbn. split; intros; try discriminate.
+  clear H1. constructor. intros ??.
+  apply (gfp_fp divergesF) in H0 as (? & ? & ?).
+  eapply dtau_match.
+  apply H0. auto.
+Qed.
+
+Inductive nodiv s : Prop :=
+| nodiv_tau : (forall s', trans tau s s' -> nodiv s') -> nodiv s
+.
+
+Lemma chain_nodiv : forall (R : Chain simF) s t,
+  nodiv s ->
+  simF `R false s t.
+Proof.
+  intro. apply tower. {
+    intros ???????. apply H; auto.
+  }
+  clear R. intros R **.
+  cbn. split; intros; try discriminate.
+  clear H1.
+  induction H0.
+  constructor. intros ??.
+  apply dtau_div. apply H1. apply H2.
+Qed.
+
+Lemma diverges_nodiv : forall s,
+  nodiv s ->
+  diverges s ->
+  False.
+Proof.
+  intros. induction H.
+  apply (gfp_fp divergesF) in H0 as (? & ? & ?).
+  apply H1 in H0 as [].
+  apply H2.
+Qed.
+
+Lemma diverges_impl_nodiv : forall s t,
+  nodiv s \/ diverges t ->
+  (diverges s -> diverges t).
+Proof.
+  intros. destruct H.
+  - now apply diverges_nodiv in H; auto.
+  - apply H.
+Qed.
+
+Definition divpres := gfp divpresF.
+
+(*Program Definition divpresF' : mon (St -> St -> Prop) :=
+{| body R s t :=
+  (forall s', trans tau s s' -> exists t', (trans tau)^+ t t' /\ R s' t') \/ nodiv s
+|}.
+Next Obligation.
+Admitted.
+
+Definition divpres' := gfp divpresF'.
+
+Lemma divpres'_divpres : forall s t, divpres' s t -> divpres s t.
+Proof.
+(*  red. coinduction R CH. intros.
+  apply (gfp_fp divpresF') in H.
+  constructor. intros ??.
+  apply H in H0 as [].
+  - destruct H0 as (? & ? & ?). admit.
+  - (* chain_nodiv *) admit.*)
+Admitted.
+(* dans l'autre sens ça va encore mal se passer *)
+
+Lemma divpres'_tau_r : forall (R : Chain divpresF') s t t',
+  trans tau t t' ->
+  `R s t' ->
+  `R s t.
+Proof.
+(*  intro. apply tower. admit. clear R. intros R ** ??.
+  apply H1 in H2 as [].
+  - left. destruct H2 as (? & ? & ?).
+    exists x. admit.
+  - right. apply H2.*)
+Admitted.*)
+
+(*Axiom extau_dec : forall s,
+  ((exists s', trans tau s s') \/ forall s', ~ trans tau s s').*)
+
+(*Lemma divpres_divpres' : forall s t, divpres s t -> divpres' s t.
+Proof.
+  red. coinduction R CH. intros.
+  apply (gfp_fp divpresF) in H. induction H.
+  intros ??. apply H in H0 as [].
+  - left. exists t'. split; auto. admit.
+  - unfold divpresF' in DIV. cbn in DIV. apply DIV.
+Abort.*)
+
+Axiom diverges_lem : forall s, diverges s \/ nodiv s.
+
+Lemma divpres_impl : forall s t,
+  divpres s t ->
+  diverges s -> diverges t.
+Proof.
+  red. coinduction R CH. intros.
+  apply (gfp_fp divpresF) in H. induction H. apply (gfp_fp divergesF) in H0 as (? & ? & ?).
+  apply H in H0 as [].
+  - exists t'. eauto.
+  - now apply DIV.
+Qed.
+
+(* ok *)
+Lemma divsim_equiv
+  (Hcompress : compress = SimOpt.compress_mut)
+  (Hlock : lock = SimOpt.nolock)
+  (Hexpand : expand = SimOpt.expand) :
+  forall b s t, divsim s t ->
+  sim b s t.
+Proof.
+  red. coinduction R CH. intros. cbn. split; intros; try discriminate.
+  { apply (gfp_fp (divsimF _)) in H. destruct H as (_ & _ & ? & _).
+    destruct (diverges_lem s).
+    apply H in H1. eapply chain_div in H1. apply H1; auto.
+    eapply chain_nodiv with (R := R) (t := t) in H1. apply H1; auto.
+
+  }
+  clear H0.
+  repeat split; intros.
+  - apply (gfp_fp (divsimF _)) in H. destruct H as (? & ? & _).
+    clear H0. assert (((trans tau)^* ⋅ trans (obs o)) s s') by admit.
+    apply H in H0 as (? & ? & ? & ? & ?).
+    eapply ans_delay_obs; eauto.
+  - apply (gfp_fp (divsimF _)) in H.
+    clear H0. assert ((trans tau)^* s s') by admit.
+    apply H in H0 as (? & ? & ?).
+    rewrite str_itr in H0. destruct H0.
+    + apply tau_div. assumption. apply CH. cbn in H0. admit.
+      admit.
+    + eapply tau_expand; eauto.
+  - admit.
+Admitted.
+
+Lemma sim_divpres : forall s t (Hcompress : compress = SimOpt.compress_mut),
+  sim true s t ->
+  gfp divpresF s t.
+Proof.
+  coinduction R CH. intros.
+  apply (gfp_fp simF) in H. destruct H as [_ ?]. specialize (H eq_refl).
+  constructor. red. intros.
+  apply H in H0 as [].
+  - eapply dtau_match; eauto.
+  - now rewrite Hcompress in H0.
+  - apply dtau_div. clear DIV. assert (DIV : gfp divpresF s' t) by admit. apply (gfp_bchain R) in DIV. apply DIV; auto.
+  - admit.
+Admitted.
+
+Lemma sim_f_t : forall s t (Hcompress : compress = SimOpt.compress_mut),
+  sim true s t ->
+  sim false s t.
+Proof.
+  red. coinduction R CH. intros.
+  split; intros; try discriminate. clear H0.
+  apply (gfp_fp simF) in H. destruct H as [_ ?]. specialize (H eq_refl).
+  constructor. red. intros.
+  apply H in H0 as [].
+  - eapply dtau_match; eauto.
+  - now rewrite Hcompress in H0.
+  - apply dtau_div. (*apply (gfp_bchain R) in DIV. apply DIV; auto.*) admit.
+  - admit.
+Admitted.
+
+Lemma simF_f_t : forall (R : Chain simF) s t (Hcompress : compress = SimOpt.compress_mut),
+  simF `R true s t ->
+  simF `R false s t.
+Proof.
+  intro. apply tower. {
+    intros ????????. apply H; auto.
+  }
+  clear R. intros R **.
+  split; intros; try discriminate. clear H1.
+  destruct H0 as [_ ?]. specialize (H0 eq_refl).
+  constructor. red. intros.
+  apply H0 in H1 as [].
+  - eapply dtau_match; eauto.
+  - now rewrite Hcompress in H1.
+  - apply dtau_div. apply DIV.
+  - admit.
+Admitted.
+
+Lemma divsim_equiv'
+  (Hcompress : compress = SimOpt.compress_mut)
+  (Hlock : lock = SimOpt.nolock)
+  (Hexpand : expand = SimOpt.expand) :
+  forall s t, (forall b, sim b s t) ->
+  divsim' s t.
+Proof.
+  red. coinduction R CH. intros. cbn -[dot str]. repeat split; intros.
+  - specialize (H true). apply (gfp_fp simF) in H. apply H in H0 as []; auto.
+    + exists o', t'. split. admit. split; auto. apply CH. intros. destruct b; auto.
+      now apply sim_f_t.
+    + admit.
+  - specialize (H true). apply (gfp_fp simF) in H. apply H in H0 as []; auto.
+    + exists t'. split. admit. apply CH. intros. destruct b; auto. now apply sim_f_t.
+    + now rewrite Hcompress in H0.
+    + exists t. split. admit. apply CH. intros []; try easy. admit.
+    + admit.
+  - specialize (H false). revert s t H H0. clear R CH. red. coinduction R CH. intros.
+    cbn. apply (gfp_fp simF) in H. pose proof (proj1 H eq_refl). clear H. revert H0. induction H1. intros.
+    apply (gfp_fp divergesF) in H0 as (? & ? & ?). apply H in H0. destruct H0; eauto.
+    destruct DIV. apply H2 in H1 as (? & ? & ?). eauto.
+Admitted.
+
+Lemma sim_tau_l (R : Chain simF) (Hcompress : compress = SimOpt.compress_mut) : forall s t,
+  is_tau_state s ->
+  (forall s', trans tau s s' -> `R true s' t) ->
+  `R true s t.
+Proof.
+  apply tower. {
+    intros ????????. apply H; auto.
+    intros. apply H1; auto.
+  }
+  clear R. intros R **.
+  split; intro; try discriminate; clear H2.
+  - repeat split; intros. 3: admit.
+    + now apply H0 in H2.
+    + apply H1 in H2. apply tau_div; auto. apply (b_chain R). apply H2.
+      apply simF_f_t; auto.
+Admitted.
 
 Section SimUpTo.
 
@@ -346,7 +688,7 @@ Context (*(div : SimOpt.div_opt) (lock : SimOpt.lock_opt)
   (exp : SimOpt.exp_opt) (ub : SimOpt.ub_opt)*)
   (R : Chain simF).
 
-Definition upto_refl `{Reflexive _ Robs} :
+(*Definition upto_refl `{Reflexive _ Robs} :
   Reflexive `R.
 Proof.
   apply tower.
@@ -354,7 +696,7 @@ Proof.
   - repeat split; intros; auto.
     + eauto 8 with optsim.
     + eauto with optsim.
-Qed.
+Qed.*)
 
 (*Lemma diverges_taustar :
   forall s s', diverges s' -> taustar s s' -> diverges s.
@@ -373,12 +715,12 @@ Proof.
 Qed.*)
 
 (* adds a tau on the right *)
-Theorem upto_tau_r' :
+(*Theorem upto_tau_r' :
   forall s t t'
     (Hcompress : compress = SimOpt.compress_coind),
   (trans tau t t' /\ forall l t'', trans l t t'' -> l = tau /\ t'' = t') ->
-  `R s t ->
-  `R s t'.
+  `R true s t ->
+  `R true s t'.
 Proof.
   apply tower. {
     intros ? INC s t t' ?????. red.
@@ -397,14 +739,14 @@ Proof.
       rewrite itr_str_l in TR. rewrite <- dotA in TR. destruct TR as [t0 TR1 TR2].
       apply H2 in TR1 as [_ ->]. apply TR2.
   + (* tau*)
-    intros. destruct H1. apply H1 in H3 as [].
+    intros. apply H1 in H3 as [].
     * apply H2 in TR as [_ ->]. econstructor 2; eauto.
     * econstructor 2; eauto.
     * now rewrite Hcompress in H3.
     * rewrite itr_str_l in TR. destruct TR as [t0 TR1 TR2].
       apply H2 in TR1 as [_ ->]. eapply tau_weak; eauto. typeclasses eauto.
   + (* deadlock *)
-    destruct H1 as [(_ & _ & [])]; auto.
+    destruct H1 as (_ & _ & []); auto.
     right. intro. apply H1 in H3. intro. eauto with optsim.
 Qed.
 
@@ -420,7 +762,7 @@ Proof.
     eapply INC; eauto.
     now apply H1.
   }
-  intros. revert t H0 H1. induction H2. repeat split; intros; subst.
+  intros. repeat split; intros; subst.
   + (* observable event *)
     apply H0 in H3 as [].
     * eleft; eauto. now apply H2 in TR as [? _].
@@ -441,14 +783,14 @@ Proof.
     right. intros. apply H0 in H3.
     intro. apply H3. econstructor; eapply H2.
 Admitted.
-
+*)
 Theorem upto_tau_r :
   forall s t t'
     (Hstuck : extrans s \/ lock = SimOpt.nolock) (* \/ taustar_det t t' *)
     (Hexpand : expand = SimOpt.expand),
   (trans tau)^* t t' ->
-  `R s t' ->
-  `R s t.
+  `R true s t' ->
+  `R true s t.
 Proof.
   apply tower. {
     intros ? INC s t t' ??????. red.
@@ -457,24 +799,25 @@ Proof.
     apply leq_infx in H1.
     now apply H1.
   }
-  intros. repeat split; intros; subst.
+  intros.
+  split; intros; try discriminate. clear H2.
+  repeat split; intros; subst.
   + (* observable event *)
-    destruct H1. apply H1 in H2 as [].
+    destruct H1 as [_ ?]. specialize (H1 eq_refl). apply H1 in H2 as [].
     * eright; eauto. esplit; eauto.
     * eright; auto. 2: apply SIM. 2: apply OBS. destruct TR. esplit. 2: apply H4.
       rewrite <- str_trans. esplit; eassumption.
   + (* tau *)
-    destruct H1. apply H1 in H2 as [].
+    destruct H1 as [_ ?]. specialize (H1 eq_refl). apply H1 in H2 as [].
     * econstructor 4; eauto.
       rewrite itr_str_r. esplit; eauto.
-    * eapply tau_weak; eauto with optsim. typeclasses eauto.
+    * (*eapply tau_weak; eauto with optsim. typeclasses eauto.*) admit.
     * eapply tau_weak_div; eauto with optsim.
       epose proof simF_eq.
-      assert (forall R : St -> St -> Prop,
-      Proper (Eq St ==> Eq St ==> iff) R ->
-      Proper (Eq St ==> Eq St ==> impl) (simInd R)) by admit. Search Proper impl iff.
-      apply proper_sym_impl_iff_2; try typeclasses eauto.
-      red. intros. now step.
+      assert (forall R : bool -> St -> St -> Prop,
+      Proper (eq ==> Eq St ==> Eq St ==> iff) R ->
+      Proper (eq ==> Eq St ==> Eq St ==> impl) (simF R)) by admit.
+      apply proper_sym_impl_iff_2; try typeclasses eauto. admit. admit.
     * econstructor 4; eauto.
       rewrite itr_str_r, <- str_trans, <- dotA, <- itr_str_r.
       esplit; eauto.
@@ -488,40 +831,41 @@ Theorem inv_tau_l :
   forall s s' t
     (Hexpand : expand = SimOpt.expand),
   trans tau s s' ->
-  simF `R s t ->
-  `R s' t.
+  simF `R true s t ->
+  `R true s' t.
 Proof.
-  intros. apply sim_alt_equiv in H0.
+  (*intros. apply sim_alt_equiv in H0.
   destruct H0 as [SIM STUCK].
   apply SIM in H as [].
   - eapply upto_tau_r; eauto. admit. now rewrite <- str_ext.
   - apply SIM0.
   - step. apply SIM0.
-  - eapply upto_tau_r; eauto. admit. rewrite str_itr. now right.
+  - eapply upto_tau_r; eauto. admit. rewrite str_itr. now right.*)
+  (* FIXME check *)
 Admitted.
 
 End SimUpTo.
 End SimDef.
 
 Theorem sim_tau_r :
-  forall compress lock s t t'
+  forall compress lock ub s t t'
     (Hstuck : extrans s \/ lock = SimOpt.nolock) (* \/ taustar_det t t' *),
   (trans tau)^* t t' ->
-  sim compress lock SimOpt.expand s t' ->
-  sim compress lock SimOpt.expand s t.
+  sim compress lock SimOpt.expand ub true s t' ->
+  sim compress lock SimOpt.expand ub true s t.
 Proof.
-  unfold sim. intros ??. apply gfp_prop.
-  intros. eapply upto_tau_r; eauto. apply SimOpt.noub.
+  unfold sim. intros ???. apply gfp_prop.
+  intros. eapply upto_tau_r; eauto.
 Qed.
 
 Theorem sim_inv_tau_l :
-  forall compress lock s s' t,
+  forall compress lock ub s s' t,
   trans tau s s' ->
-  sim compress lock SimOpt.expand s t ->
-  sim compress lock SimOpt.expand s' t.
+  sim compress lock SimOpt.expand ub true s t ->
+  sim compress lock SimOpt.expand ub true s' t.
 Proof.
-  unfold sim. intros. apply (gfp_fp (simF _ _ _)) in H0. revert H0. eapply gfp_prop.
-  intros. eapply inv_tau_l; eauto. constructor.
+  unfold sim. intros. apply (gfp_fp (simF _ _ _ _)) in H0. revert H0. eapply gfp_prop.
+  intros. eapply inv_tau_l; eauto.
 Qed.
 
 Lemma srel_str_ind_l' {E : EqType} :
@@ -540,13 +884,13 @@ Proof.
 Qed.
 
 Theorem sim_inv_taustar_l :
-  forall compress lock s s' t,
+  forall compress lock ub s s' t,
   (trans tau)^* s s' ->
-  sim compress lock SimOpt.expand s t ->
-  sim compress lock SimOpt.expand s' t.
+  sim compress lock SimOpt.expand ub true s t ->
+  sim compress lock SimOpt.expand ub true s' t.
 Proof.
   intros. revert H0.
-  eapply srel_str_ind_l' with (i := trans tau) (P := fun s s' => sim _ _ _ s t -> sim _ _ _ s' t); auto.
+  eapply srel_str_ind_l' with (i := trans tau) (P := fun s s' => sim _ _ _ _ true s t -> sim _ _ _ _ true s' t); auto.
   - cbn. intros. now rewrite H0, H1.
   - intros. rewrite <- H0. apply H1.
   - intros. apply H1. eapply sim_inv_tau_l; eauto.
@@ -619,137 +963,158 @@ Proof.
 Qed.
 
 
-Lemma sim_diverges : forall lock expand s t,
-  sim SimOpt.compress_ind lock expand s t ->
+Lemma sim_diverges : forall lock expand ub s t,
+  sim SimOpt.compress_mut lock expand ub true s t ->
   diverges s ->
   diverges t.
 Proof.
-  red. coinduction R CH.
-  intros. apply (gfp_fp (simF _ _ _)) in H. revert H0. induction H.
-  intros.
-  apply (gfp_fp divergesF) in H0 as (? & ? & ?).
-  apply H in H0. destruct H0.
-  - exists t'; split; eauto.
-  - discriminate.
-  - destruct SIM. eauto.
-  - eapply divergesF_tauplus; eauto.
+  intros. eapply divpres_impl; eauto. eapply sim_divpres; eauto.
+Qed.
+
+Lemma sim_tau_weak :
+  forall compress lock expand ub s s' t R,
+  simF compress lock expand ub R true s t ->
+  trans tau s s' ->
+  exists t', (trans tau)^* t t' /\ R true s' t'.
+Proof.
+  intros. apply H in H0 as []; auto.
+  - exists t'. split; auto. now rewrite <- str_ext.
+  - exists t. split; auto. now rewrite <- str_refl.
+  - exists t. split; auto. now rewrite <- str_refl.
+  - exists t'. split; auto. now rewrite <- str_itr'.
 Qed.
 
 Hint Constructors ObsAnswer : optsim.
 Hint Constructors TauAnswer : optsim.
 
-Lemma sim_tau_weak :
-  forall compress lock expand (Hcompress : compress <> SimOpt.compress_ind) s s' t R,
-  simF compress lock expand R s t ->
-  trans tau s s' ->
-  exists t', (trans tau)^* t t' /\ R s' t'.
+Lemma diverges_divpres :
+  forall s t, diverges t -> divpres s t.
 Proof.
-  intros. apply H in H0 as [].
-  - exists t'. split; auto. now rewrite <- str_ext.
-  - exists t. split; auto. now rewrite <- str_refl.
-  - easy.
-  - exists t'. split; auto. now rewrite <- str_itr'.
+  red. coinduction R CH.
+  intros. constructor. intros ??.
+  apply (gfp_fp divergesF) in H as (? & ? & ?).
+  eleft; eauto.
+Qed.
+
+Lemma divpres_nocompress_r : forall lock expand ub (R : Chain (simF SimOpt.compress_mut lock expand ub)) s t u,
+  `R false s t ->
+  sim SimOpt.nocompress lock expand ub true t u ->
+  `R false s u.
+Proof.
+  intros ????. apply tower. {
+    intros ?????????. eapply H; eauto.
+  }
+  clear R. intros R **.
+  destruct H0 as [? _]. specialize (H0 eq_refl). induction H0. constructor. intros _. constructor. intros ??. apply H0 in H2 as [].
+  - apply (gfp_fp (simF _ _ _ _)) in H1. apply H1 in TR as []; auto.
+    + eleft. apply TR. eapply H. apply DIV. apply SIM.
+    + discriminate.
+    + discriminate.
+    + subst. admit.
+  - right. apply DIV in H1. apply H1; auto.
+Admitted.
+
+Lemma divpres_trans_l : forall compress lock expand ub (R : Chain (simF compress lock expand ub)) s t u,
+  `R false t u ->
+  divpres s t ->
+  `R false s u.
+Proof.
+  intros ?????. apply tower. {
+    intros ?????????. eapply H; eauto.
+  }
+  clear R. intros R **.
+  destruct H0 as [? _]. specialize (H0 eq_refl).
+  revert s H1. induction H0. rename t into u. rename s into t. intros.
+  apply (gfp_fp divpresF) in H1. induction H1.
+  constructor; intros; try discriminate. clear H2. constructor. intros ??.
+  apply H1 in H2 as ?. destruct H3.
+  - apply H0 in TR. destruct TR.
+    + rename t'0 into u'. eapply dtau_match; eauto.
+    + apply dtau_div. apply DIV0 in DIV. apply DIV; auto.
+  - apply dtau_div. apply DIV; auto.
 Qed.
 
 Theorem upto_sim_r :
-  forall compress lock expand (R : Chain (simF compress lock expand)) s t t'
+  forall compress lock expand ub (R : Chain (simF compress lock expand ub)) s t t'
     (OBS : Transitive Robs),
-  `R s t' ->
-  sim (match compress with SimOpt.compress_ind => SimOpt.nocompress | _ => compress end) lock expand t' t ->
-  `R s t.
+  `R true s t' ->
+  sim (match compress with SimOpt.compress_mut => SimOpt.nocompress | _ => compress end) lock expand ub true t' t ->
+  `R true s t.
 Proof.
-  intros ????.
+  intros ?????.
   apply tower. {
     intros ??????????. red.
     eapply H; eauto.
     apply leq_infx in H2. apply H2, H0.
   }
-  intros. revert t H1. induction H0.
+  intros.
+  split; intros; try discriminate. clear H2.
   repeat split; intros; subst.
-  - apply H0 in H2 as [].
-    + apply (gfp_fp (simF _ _ _)) in H1. destruct H1.
+  - apply H0 in H2 as []; auto.
+    + apply (gfp_fp (simF _ _ _ _)) in H1. destruct H1 as [_ ?]. specialize (H1 eq_refl).
       apply H1 in TR. destruct TR; eauto with optsim.
     + destruct TR as [t'' TR1 TR2].
       subst. eapply sim_inv_taustar_l in H1; eauto.
-      apply (gfp_fp (simF _ _ _)) in H1.
-      apply H1 in TR2. destruct TR2; eauto with optsim.
-  - apply H0 in H2 as [].
-    + (* tau_exact *) apply (gfp_fp (simF _ _ _)) in H1. destruct H1.
+      apply (gfp_fp (simF _ _ _ _)) in H1.
+      apply H1 in TR2; auto. destruct TR2; eauto with optsim.
+  - apply H0 in H2 as []; auto.
+    + (* tau_exact *) apply (gfp_fp (simF _ _ _ _)) in H1. destruct H1 as [_ ?]. specialize (H1 eq_refl).
       apply H1 in TR as ?. destruct H2; eauto with optsim.
       * (* compress_coind *) destruct compress; try discriminate. apply tau_compress; auto. eapply H; eauto.
       * (* compress_ind *) destruct compress; discriminate.
     + (* tau_compress *) subst compress.
       eapply tau_compress; eauto.
     + (* tau_div *) subst compress.
-      eapply tau_div; auto.
-      now apply SIM.
+      eapply tau_div; eauto with optsim. assert (simF SimOpt.compress_mut lock expand ub `x false s' t).  eapply divpres_nocompress_r. split. intros _. apply DIV. now intro. apply H1. now apply H2.
     + (* tau_expand *)
       rewrite itr_str_r in TR. destruct TR as [t'1 TR1 TR2].
       subst.
       eapply sim_inv_taustar_l in H1; eauto.
-      apply (gfp_fp (simF _ _ _)) in H1.
-      apply H1 in TR2.
+      apply (gfp_fp (simF _ _ _ _)) in H1.
+      apply H1 in TR2; auto.
       destruct compress; destruct TR2; try discriminate; eauto with optsim.
-  - destruct H0. apply (gfp_fp (simF _ _ _)) in H1 as [(_ & _ & ?)]. intuition.
+  - destruct H0. apply (gfp_fp (simF _ _ _ _)) in H1 as (_ & _ & ?); auto. intuition.
 Qed.
 
-(* direct definition of divergence-sensitive weak simulation *)
-Program Definition divsimF lock : mon (St -> St -> Prop) :=
-{|
-  body := fun R s t => (forall o s', ((trans tau)^* ⋅ trans (obs o)) s s' ->
-    exists o' t',
-        ((trans tau)^* ⋅ trans (obs o')) t t' /\
-      R s' t' /\
-      Robs o o') /\
-  (forall s', (trans tau)^* s s' ->
-    exists t', 
-      (trans tau)^* t t' /\ R s' t') /\
-  (diverges s -> diverges t) /\
-  (lock = SimOpt.nolock \/ (is_stuck s -> is_stuck t))
-|}.
-Next Obligation.
-  repeat split; intros; auto.
-  - apply H0 in H4 as (? & ? & ? & ? & ?). eauto 6.
-  - apply H1 in H4 as (? & ? & ?). eauto.
-Qed.
-
-Lemma divsim_equiv :
-  forall s t, sim SimOpt.compress_ind SimOpt.nolock SimOpt.expand s t ->
-  gfp (divsimF SimOpt.nolock) s t.
+Theorem upto_sim_l :
+  forall compress lock expand ub (R : Chain (simF compress lock expand ub)) s s' t
+    (OBS : Transitive Robs),
+  `R true s' t ->
+  sim compress lock SimOpt.noexpand ub true s s' ->
+  `R true s t.
 Proof.
-  intros. apply (gfp_fp (divsimF _)).
-  repeat split; intros.
-  - admit.
-  - admit.
-  - intros. now apply sim_diverges in H.
-  - auto.
-Admitted.
-
-
-(*Theorem upto_sim_l :
-  forall s s' t (Hstuck : extrans s \/ lock = SimOpt.nolock),
-  `R s' t ->
-  wsim div lock exp ub s s' ->
-  `R s t.
-Proof.
-  apply tower.
-  - intros ??????????. red.
+  intros ?????.
+  apply tower. {
+    intros ??????????. red.
     eapply H; eauto.
     apply leq_infx in H2. apply H2, H0.
-  - intros. repeat split; intros; subst.
-    + apply (gfp_fp (wsimF _ _ _ _)) in H1.
-      apply H1 in H2 as (? & ? & ? & ? & ?).
-      admit.
-    + apply (gfp_fp (wsimF _ _ _ _)) in H1.
-      apply H1 in H2 as (? & ? & ?).
-      clear H2. assert (H2 : trans tau s' x0) by admit.
-      apply H0 in H2 as (? & ? & ?).
-      exists x1. split; auto.
-      (* problem if H2 is the identity *)
-      admit.
-Abort.
+  }
+  intros.
+  split; intros; try discriminate. clear H2.
+  repeat split; intros; subst.
+  - apply (gfp_fp (simF _ _ _ _)) in H1. destruct H1 as [_ ?]. specialize (H1 eq_refl).
+    apply H1 in H2 as [].
+    + apply H0 in TR; auto. destruct TR; eauto with optsim.
+    + discriminate.
+  - apply (gfp_fp (simF _ _ _ _)) in H1. destruct H1 as [_ ?]. specialize (H1 eq_refl).
+    apply H1 in H2 as [].
+    + (* tau_exact *)
+      apply H0 in TR as ?; auto. destruct H2; eauto with optsim.
+      (* compress_mut *) subst. apply tau_div; eauto.
+      assert (simF SimOpt.compress_mut lock expand ub `x false s'0 t). eapply divpres_trans_l with (t := t'). split; intro; try discriminate. apply DIV. admit.
+      apply H2; auto.
+    + (* tau_compress *) subst compress.
+      eapply tau_compress; eauto. eapply H; eauto. apply (b_chain x). apply H0.
+    + (* tau_div *) subst compress.
+      eapply tau_div; eauto with optsim.
+      eapply H; eauto. apply (b_chain x). apply H0.
+      apply simF_f_t in H0; auto. apply divpres_trans_l with (s := s'0) in H0. now apply H0. admit.
+    + (* tau_expand *)
+      discriminate.
+  - destruct H0. apply (gfp_fp (simF _ _ _ _)) in H1 as (_ & _ & ?); auto. intuition.
+Admitted.
 
-
+(*
 Lemma wsim_obs' :
   forall s t
     (Hstuck : extrans s \/ lock = SimOpt.nolock),
